Packwork

DeBruijnSSA/BinSyntax/Rewrite/Term/Compose/Structural.lean
@@ -28,31 +28,52 @@ theorem Eqv.pack_sum_def {Γ : Ctx α ε} {R : LCtx α} {i : Fin R.length}
       ext
       simp [Term.pack0, Term.Wf.pack0, -Function.iterate_succ, Function.iterate_succ']
 
-def Eqv.pack' {Γ : Ctx α ε} : Eqv φ Γ (Γ.pack, Γ.sup_effect) := match Γ with
-  | [] => unit ⊥
-  | V::Γ => pair (var 0 (by cases V; simp)) ((pack' (Γ := Γ)).wk0.wk_eff (by simp))
+def Eqv.pack {Γ : Ctx α ε} (h : ∀i, Γ.effect i ≤ e) : Eqv φ Γ (Γ.pack, e) := match Γ with
+  | [] => unit e
+  | V::Γ => pair
+    (var 0 (Ctx.Var.head (by constructor; rfl; convert (h 0); simp) _))
+    ((pack (Γ := Γ) (λi => by convert h (i + 1) using 1; simp)).wk0)
 
-theorem Eqv.pack_def' {Γ : Ctx α ε} : Eqv.pack' (φ := φ) (Γ := Γ) = ⟦Term.InS.pack'⟧ := by
+theorem Eqv.pack_def {Γ : Ctx α ε} {h : ∀i, Γ.effect i ≤ e}
+  : Eqv.pack (φ := φ) (Γ := Γ) h = ⟦Term.InS.pack h⟧ := by
   induction Γ with
   | nil => rfl
-  | cons _ _ I => simp only [pack', I]; rfl
+  | cons _ _ I => simp only [pack, I]; rfl
 
-def _root_.BinSyntax.Ctx.Pure.packE' {Γ : Ctx α ε} (h : Γ.Pure) : Eqv φ Γ (Γ.pack, ⊥) := match Γ with
-  | [] => Eqv.unit ⊥
-  | V::Γ => Eqv.pair (Eqv.var 0 (by cases V; convert h.head; simp)) h.tail.packE'.wk0
+abbrev _root_.BinSyntax.Ctx.Pure.packE {Γ : Ctx α ε} (h : Γ.Pure) : Eqv φ Γ (Γ.pack, ⊥)
+  := Eqv.pack (e := ⊥) (h := λi => by simp [h.effect i])
 
-theorem Eqv.packE_def' {Γ : Ctx α ε} {h : Γ.Pure} : h.packE' (φ := φ) = ⟦h.pack'⟧ := by
-  induction Γ with
-  | nil => rfl
-  | cons _ _ I => simp only [Ctx.Pure.packE', I]; rfl
+theorem Eqv.packE_def' {Γ : Ctx α ε} {h : Γ.Pure} : h.packE (φ := φ) = ⟦h.pack⟧ := by
+  simp only [Ctx.Pure.packE, pack_def]
+
+@[simp]
+theorem Eqv.wk_eff_pack {Γ : Ctx α ε} {h : ∀i, Γ.effect i ≤ lo} {h' : lo ≤ hi}
+  : (pack (φ := φ) h).wk_eff h' = pack (λi => (h i).trans h') := by
+  simp [pack_def]
+
+theorem Eqv.wk_eff_packE {Γ : Ctx α ε} {h : Γ.Pure}
+  : h.packE.wk_eff bot_le = pack (φ := φ) (e := hi) (λi => by simp [h.effect]) := by simp
+
+@[simp]
+theorem  _root_.BinSyntax.Ctx.Pure.packP {Γ : Ctx α ε} (h : Γ.Pure) (h')
+  : Eqv.Pure (Eqv.pack (φ := φ) (Γ := Γ) (e := e) h')
+  := ⟨h.packE, by simp⟩
 
 def Eqv.pack_drop {Γ Δ : Ctx α ε} (i : Fin Γ.length)
   : Eqv φ ((Γ.pack, ⊥)::Δ) (Ctx.pack (Γ.drop i), e)
   := ⟦InS.pack_drop i⟧
 
+theorem Eqv.Pure.pack_drop {Γ Δ : Ctx α ε} {i : Fin Γ.length}
+  : Pure (pack_drop (φ := φ) (Δ := Δ) (e := e) i)
+  := ⟨Eqv.pack_drop i, rfl⟩
+
 def Eqv.pack_drop' {Γ Δ : Ctx α ε} (i : Fin Γ.length)
   : Eqv φ ((Γ.pack, ⊥)::Δ) ((Γ.get i).1.prod (Ctx.pack (Γ.drop (i + 1))), e)
   := ⟦InS.pack_drop' i⟧
+
+theorem Eqv.Pure.pack_drop' {Γ Δ : Ctx α ε} {i : Fin Γ.length}
+  : Pure (pack_drop' (φ := φ) (Δ := Δ) (e := e) i)
+  := ⟨Eqv.pack_drop' i, rfl⟩
 
 theorem Eqv.cast_pack_drop {Γ Δ : Ctx α ε} {i : Fin Γ.length}
   : (Eqv.pack_drop (φ := φ) (Δ := Δ) (e := e) i).cast rfl (by rw [Ctx.pack_drop_fin]) = pack_drop' i
@@ -70,6 +91,10 @@ def Eqv.pack_drop_succ {Γ Δ : Ctx α ε} (i : Fin Γ.length)
 
 def Eqv.unpack0 {Γ Δ : Ctx α ε} (i : Fin Γ.length) : Eqv φ ((Γ.pack, ⊥)::Δ) ((Γ.get i).1, e)
   := ⟦InS.unpack0 i⟧
+
+theorem Eqv.Pure.unpack0 {Γ Δ : Ctx α ε} {i : Fin Γ.length}
+  : Pure (unpack0 (φ := φ) (Δ := Δ) (e := e) i)
+  := ⟨Eqv.unpack0 i, rfl⟩
 
 theorem Eqv.pl_pack_drop'  {Γ Δ : Ctx α ε} {i : Fin Γ.length}
   : (Eqv.pack_drop' (φ := φ) (Δ := Δ) (e := e) i).pl = unpack0 i := rfl
@@ -94,6 +119,34 @@ theorem Eqv.unpack0_def' {Γ Δ : Ctx α ε} (i : Fin Γ.length) :
       List.getElem_cons_zero, I, InS.unpack0'
     ]
     cases i using Fin.cases <;> rfl
+
+def Subst.Eqv.unpack {Γ Δ : Ctx α ε} : Subst.Eqv φ ((Γ.pack, ⊥)::Δ) Γ := ⟦Subst.InS.unpack⟧
+
+def Eqv.packed {Γ Δ : Ctx α ε} (a : Eqv φ Γ V) : Eqv φ ((Γ.pack, ⊥)::Δ) V
+  := a.subst Subst.Eqv.unpack
+
+def Eqv.unpacked {Γ : Ctx α ε} (a : Eqv φ [(Γ.pack, ⊥)] (A, e)) (h : ∀i, Γ.effect i ≤ e)
+  : Eqv φ Γ (A, e) := let1 (pack h) (a.wk_id (by simp [Ctx.Wkn.drop]))
+
+-- theorem Eqv.packed_unpacked {Γ : Ctx α ε} {a : Eqv φ [(Γ.pack, ⊥)] (A, e)} (h : Γ.Pure)
+--   : (a.unpacked (λi => by simp [h.effect])).packed = a := by
+--   rw [
+--     unpacked, <-wk_eff_packE (h := h), let1_beta, packed, subst_subst, <-wk_eq_wk_id,
+--     <-subst_fromWk, subst_subst, subst_id'
+--   ]
+--   ext k; cases k using Fin.elim1
+--   simp only [Fin.isValue, List.get_eq_getElem, List.length_singleton, Fin.val_zero,
+--     List.getElem_cons_zero, Set.mem_setOf_eq, Subst.Eqv.get_comp, Subst.Eqv.get_fromWk,
+--     Fin.zero_eta, Fin.coe_fin_one, id_eq, subst_var, List.length_cons, subst0_get_zero,
+--      wk_res_self,
+--     Subst.Eqv.get_id, Ctx.Pure.packE]
+--   induction Γ with
+--   | nil => apply Eqv.terminal
+--   | cons V Γ I =>
+--     simp [Eqv.pack, subst_var]
+--     convert Eqv.Pure.pair_eta ⟨var 0 Ctx.Var.shead, rfl⟩
+--     simp only [wk_eff_self]
+--     sorry
 
 -- theorem Eqv.unpack0_eq_unpack0' {Γ Δ : Ctx α ε} (i : Fin Γ.length) :
 --   Eqv.unpack0 (φ := φ) (Δ := Δ) (e := e) i = Eqv.unpack0' i := by
